simplify implementations using cvariable autoallocation.

src/Verse/CryptoLib/blake2s/c/portable.v
@@ -39,72 +39,19 @@ Inductive name := verse_blake2s_c_portable_iter | verse_blake2s_c_portable_last.
 
 Require Verse.CryptoLib.blake2.
 
-
-Module Allocation.
-
-  Definition cword := uint32_t.
-
-  Axiom blockPtr : cvar (ptrToArray blake2.BLOCK_SIZE cword).
-  Axiom nBlocks  : cvar uint64_t.
-  Axiom UpperRef LowerRef : cvar (array 1 cword).
-
-  Axiom lastBlock : cvar (array blake2.BLOCK_SIZE cword).
-  Axiom nBytes   : cvar uint64_t.
-  Axiom Upper Lower : cvar cword.
-  Axiom f0 f1 : cvar cword.
-
-  Axiom hash     : cvar (ptrToArray blake2.HASH_SIZE cword).
-  Axiom h0 h1 h2 h3 h4 h5 h6 h7 : cvar cword.
-  Axiom w0 w1 w2 w3 w4 w5 w6 w7 w8 w9 w10 w11 w12 w13 w14 w15 : cvar cword.
-  Axiom v0 v1 v2 v3 v4 v5 v6 v7 v8 v9 v10 v11 v12 v13 v14 v15 : cvar cword.
-  Axiom C LMSB U L : cvar cword.
-End Allocation.
-
-Export Allocation.
-
-Definition params     := (- UpperRef , LowerRef , hash -).
-Definition paramsLast := (- lastBlock, nBytes, Upper, Lower, f0, f1, hash -).
-
-Definition locals     := (- h0 , h1 , h2 , h3 , h4 , h5 , h6 , h7 -).
-Definition registers  :=
-  (- w0 , w1 , w2 , w3 , w4 , w5 , w6 , w7 , w8 , w9 , w10 , w11 , w12 , w13,  w14 ,  w15 ,
-     v0 , v4 , v8 , v12,
-     v1 , v5 , v9 , v13,
-     v2 , v6 , v10, v14,
-     v3 , v7 , v11, v15,
-     C, LMSB, U, L
-  -).
-
-Definition registersLast  :=
-  (- w0 , w1 , w2 , w3 , w4 , w5 , w6 , w7 , w8 , w9 , w10 , w11 , w12 , w13,  w14 ,  w15 ,
-     v0 , v4 , v8 , v12,
-     v1 , v5 , v9 , v13,
-     v2 , v6 , v10, v14,
-     v3 , v7 , v11, v15,
-     C, LMSB
-  -).
-
-
 Definition blake2sIter
-  := Compile.Iterator verse_blake2s_c_portable_iter
+  := CIterator verse_blake2s_c_portable_iter
                       Blake2s.Block
                       Blake2s.paramIterator
                       Blake2s.stack
                       Blake2s.regIterator
-                      (blockPtr,nBlocks)
-                      params
-                      locals
-                      registers
                       Blake2s.Iterator.
 
 Definition blake2sLast
-  := Compile.Function verse_blake2s_c_portable_last
+  := CFunction verse_blake2s_c_portable_last
                       Blake2s.paramLastBlock
                       Blake2s.stack
                       Blake2s.regLastBlock
-                      paramsLast
-                      locals
-                      registersLast
                       Blake2s.LastBlockCompress.
 
 Require Import Verse.Error.
@@ -129,7 +76,7 @@ Arguments raazFFI [Name].
 
 Require Import Verse.Print.
 Require Import Verse.Target.C.Pretty.
-Goal to_print programLast.
+Goal to_print blake2sLast.
   print.
 Abort.
 
